theories/Escape.v
@@ -6,26 +6,27 @@ Definition escape {l Γ A} :
     [Γ ||-< l > A ] ->
     [Γ |- A].
 Proof.
-  eapply (LR_rect (fun l Γ A _ => [Γ |- A])).
-  - intros ? [].
-    mltt.
-  - intros _ ? ? [] ; cbn in *.
-    mltt.
-  - intros ? ? ? [] ; cbn in *.
-    mltt.
+  intros [[] lr].
+  cbn in lr.
+  induction lr as [? [] | ? ? [] | ? ? [] ] using LR_rect.
+  - mltt.
+  - mltt.
+  - mltt.
 Qed.
 
 Definition escapeEq {l Γ A B} (lr : [Γ ||-< l > A]) :
     [ Γ ||-< l > A ≅ B | lr ] ->
     [Γ |- A ≅ B].
 Proof.
-  eapply (LR_rect (fun l Γ A lr => forall B : term, [Γ ||-< l > A ≅ B | lr] -> [Γ |- A ≅ B])).
-  + intros ? [] ? [->].
+  destruct lr as [[] lr].
+  cbn in *.
+  induction lr as [ ? [] | ? ? [] | ? ? [] IHdom IHcod] using LR_rect.
+  + intros [->].
     mltt.
-  + intros ? ? ? [] ? [].
+  + intros [].
     do 2 eapply TypeTrans.
     all: mltt.
-  + intros ? ? ? [] _ _ _ ? [] ; cbn in *.
+  + intros [] ; cbn in *.
     do 2 eapply TypeTrans.
     all: mltt.
 Qed.
@@ -34,35 +35,35 @@ Definition escapeTerm {l Γ t A} (lr : [Γ ||-< l > A ]) :
   [Γ ||-< l > t : A | lr ] ->
   [Γ |- t : A].
 Proof.
-  eapply (LR_rect (fun l Γ A lr => forall t : term, [Γ ||-< l > t : A | lr ] -> [Γ |- t : A])).
-  - intros ? [] ? [] ; cbn in *.
-    mltt.
-  - intros ? ? ? [] ? [] ; cbn in *.
-    mltt.
-  - intros ? ? ? [] _ _ _ ? [] ; cbn in *.
-    mltt.
+  destruct lr as [[] lr].
+  cbn in *.
+  induction lr as [ ? [] | ? ? [] | ? ? [] IHdom IHcod] using LR_rect.
+  all: intros [] ; cbn in *.
+  all: mltt.
 Qed.
 
 Definition escapeEqTerm {l Γ t u A} (lr : [Γ ||-< l > A ]) :
   [Γ ||-< l > t ≅ u : A | lr ] ->
   [Γ |- t ≅ u: A].
 Proof.
-  eapply (LR_rect (fun l Γ A lr => forall t u, [Γ ||-< l > t ≅ u : A | lr] -> [Γ |- t ≅ u : A])).
-  - intros ? [] ? ? [[termL] [termR]] ; cbn in *.
+  destruct lr as [[] lr].
+  cbn in *.
+  induction lr as [ ? [] | ? ? [] | ? ? [] IHdom IHcod] using LR_rect.
+  - intros [[termL] [termR]] ; cbn in *.
     eapply (TermTrans (t' := termL)).
     1: mltt.
     eapply (TermTrans (t' := termR)).
     1: mltt.
     eapply TermConv.
     all: mltt.
-  - intros ? ? ? [] ? ? [] ; cbn in *.
+  - intros [] ; cbn in *.
     eapply (TermTrans (t' := termL)).
     1: mltt.
     eapply (TermTrans (t' := termR)).
     1: mltt.
     eapply TermConv.
     all: mltt.
-  - intros ? ? ? [] _ _ _ ? ? [[termL] [termR]] ; cbn in *.
+  - intros [[termL] [termR]] ; cbn in *.
     eapply (TermTrans (t' := termL)).
     1: mltt.
     eapply (TermTrans (t' := termR)).
