theories/Irrelevance.v
@@ -1,0 +1,443 @@
+From MetaCoq Require Import PCUICAst.
+Require Import Utils Automation Untyped MLTTTyping LogicalRelation Properties Reduction LRInduction ShapeView Reflexivity.
+
+Lemma ΠIrrelevanceTyEq Γ A A' na na' dom dom' cod cod'
+  (domTy : [Γ |- dom])
+  (codTy : [Γ,, vass na dom |- cod])
+  (red : [Γ |- A :⇒*: tProd na dom cod])
+  (domRed : forall Δ : context, [  |- Δ] -> LRPack Δ dom)
+  (codRed : forall (Δ : context) (a : term) (h : [  |- Δ]),
+            [domRed Δ h | Δ ||- a : dom] -> LRPack Δ (cod {0 := a}))
+  (codExt : forall (Δ : context) (a b : term) (h : [  |- Δ])
+              (ha : [domRed Δ h | Δ ||- a : dom]),
+            [domRed Δ h | Δ ||- b : dom] ->
+            [domRed Δ h | Δ ||- a ≅ b : dom] ->
+            [codRed Δ a h ha | Δ ||- cod{0 := a} ≅ cod{0 := b}])
+  (domTy': [Γ |- dom'])
+  (codTy': [Γ,, vass na' dom' |- cod'])
+  (red': [Γ |- A' :⇒*: tProd na' dom' cod'])
+  (domRed': forall Δ : context, [  |- Δ] -> LRPack Δ dom')
+  (codRed': forall (Δ : context) (a : term) (h : [  |- Δ]),
+            [domRed' Δ h | Δ ||- a : dom'] -> LRPack Δ (cod' {0 := a}))
+  (codExt': forall (Δ : context) (a b : term) (h : [  |- Δ])
+              (ha : [domRed' Δ h | Δ ||- a : dom']),
+            [domRed' Δ h | Δ ||- b : dom'] ->
+            [domRed' Δ h | Δ ||- a ≅ b : dom'] ->
+            [codRed' Δ a h ha | Δ ||- cod'{0 := a} ≅ cod'{0 := b}])
+  (eqPi : [Γ |- tProd na dom cod ≅ tProd na' dom' cod']) :
+  
+  (forall (Δ : context) (h : [  |- Δ]),
+  [× (forall B : term,
+      [domRed Δ h | Δ ||- dom ≅ B] <-> [domRed' Δ h | Δ ||- dom' ≅ B]),
+    (forall t : term,
+      [domRed Δ h | Δ ||- t : dom] <-> [domRed' Δ h | Δ ||- t : dom']) &
+    (forall t u : term,
+      [domRed Δ h | Δ ||- t ≅ u : dom ] <-> [domRed' Δ h | Δ ||- t ≅ u : dom'])]) ->
+  (forall (Δ : context) (a : term) (h : [  |- Δ])
+      (ha : [domRed Δ h | Δ ||- a : dom])
+      (ha' : [domRed' Δ h | Δ ||- a : dom']),
+  [× (forall B : term,
+      [codRed Δ a h ha | Δ ||- cod{0 := a} ≅ B] <->
+      [codRed' Δ a h ha' | Δ ||- cod'{0 := a} ≅ B]),
+    (forall t : term,
+      [codRed Δ a h ha | Δ ||- t : cod{0 := a} ] <->
+      [codRed' Δ a h ha' | Δ ||- t : cod'{0 := a} ]) &
+    (forall t u : term,
+      [codRed Δ a h ha | Δ ||- t ≅ u : cod{0 := a} ] <->
+      [codRed' Δ a h ha' | Δ ||- t ≅ u : cod'{0 := a} ])]) ->
+  let ΠA : PiRedTy Γ A := {|
+      PiRedTy.na := na ; PiRedTy.dom := dom ;
+      PiRedTy.cod := cod ;
+      PiRedTy.red := red ;
+      PiRedTy.domTy := domTy ;
+      PiRedTy.codTy := codTy ;
+      PiRedTy.domRed := domRed ;
+      PiRedTy.codRed := codRed ;
+      PiRedTy.codExt := codExt
+        |} in
+  let ΠA' : PiRedTy Γ A' := {|
+    PiRedTy.na := na' ; PiRedTy.dom := dom' ;
+    PiRedTy.cod := cod' ;
+    PiRedTy.red := red' ;
+    PiRedTy.domTy := domTy' ;
+    PiRedTy.codTy := codTy' ;
+    PiRedTy.domRed := domRed' ;
+    PiRedTy.codRed := codRed' ;
+    PiRedTy.codExt := codExt'
+      |} in
+  forall B, [Γ ||-Π A ≅ B | ΠA] -> [Γ ||-Π A' ≅ B | ΠA'].
+Proof.
+  intros IHdom IHcod ΠA ΠA' B [] ; cbn in *.
+  econstructor.
+  1-2: now mltt.
+  1: intros ; now apply IHdom.
+  intros.
+  cbn in *.
+  unshelve eapply IHcod.
+  2: eauto.
+  now eapply IHdom.
+Qed.
+
+Lemma ΠIrrelevanceTm Γ A na dom cod A' na' dom' cod'
+  (domTy : [Γ |- dom])
+  (codTy : [Γ,, vass na dom |- cod])
+  (red : [Γ |- A :⇒*: tProd na dom cod])
+  (domRed : forall Δ : context, [  |- Δ] -> LRPack Δ dom)
+  (codRed : forall (Δ : context) (a : term) (h : [  |- Δ]),
+            [domRed Δ h | Δ ||- a : dom] -> LRPack Δ (cod {0 := a}))
+  (codExt : forall (Δ : context) (a b : term) (h : [  |- Δ])
+              (ha : [domRed Δ h | Δ ||- a : dom]),
+            [domRed Δ h | Δ ||- b : dom] ->
+            [domRed Δ h | Δ ||- a ≅ b : dom] ->
+            [codRed Δ a h ha | Δ ||- cod{0 := a} ≅ cod{0 := b}])
+  (domTy': [Γ |- dom'])
+  (codTy': [Γ,, vass na' dom' |- cod'])
+  (red': [Γ |- A' :⇒*: tProd na' dom' cod'])
+  (domRed': forall Δ : context, [  |- Δ] -> LRPack Δ dom')
+  (codRed': forall (Δ : context) (a : term) (h : [  |- Δ]),
+            [domRed' Δ h | Δ ||- a : dom'] -> LRPack Δ (cod' {0 := a}))
+  (codExt': forall (Δ : context) (a b : term) (h : [  |- Δ])
+              (ha : [domRed' Δ h | Δ ||- a : dom']),
+            [domRed' Δ h | Δ ||- b : dom'] ->
+            [domRed' Δ h | Δ ||- a ≅ b : dom'] ->
+            [codRed' Δ a h ha | Δ ||- cod'{0 := a} ≅ cod'{0 := b}])
+  (eqPi : [Γ |- tProd na dom cod ≅ tProd na' dom' cod']) :
+  
+  (forall (Δ : context) (h : [  |- Δ]),
+  [× (forall B : term,
+      [domRed Δ h | Δ ||- dom ≅ B] <-> [domRed' Δ h | Δ ||- dom' ≅ B]),
+    (forall t : term,
+      [domRed Δ h | Δ ||- t : dom] <-> [domRed' Δ h | Δ ||- t : dom']) &
+    (forall t u : term,
+      [domRed Δ h | Δ ||- t ≅ u : dom ] <-> [domRed' Δ h | Δ ||- t ≅ u : dom'])]) ->
+  (forall (Δ : context) (a : term) (h : [  |- Δ])
+      (ha : [domRed Δ h | Δ ||- a : dom])
+      (ha' : [domRed' Δ h | Δ ||- a : dom']),
+  [× (forall B : term,
+      [codRed Δ a h ha | Δ ||- cod{0 := a} ≅ B] <->
+      [codRed' Δ a h ha' | Δ ||- cod'{0 := a} ≅ B]),
+    (forall t : term,
+      [codRed Δ a h ha | Δ ||- t : cod{0 := a} ] <->
+      [codRed' Δ a h ha' | Δ ||- t : cod'{0 := a} ]) &
+    (forall t u : term,
+      [codRed Δ a h ha | Δ ||- t ≅ u : cod{0 := a} ] <->
+      [codRed' Δ a h ha' | Δ ||- t ≅ u : cod'{0 := a} ])]) ->
+  let ΠA : PiRedTy Γ A := {|
+      PiRedTy.na := na ; PiRedTy.dom := dom ;
+      PiRedTy.cod := cod ;
+      PiRedTy.red := red ;
+      PiRedTy.domTy := domTy ;
+      PiRedTy.codTy := codTy ;
+      PiRedTy.domRed := domRed ;
+      PiRedTy.codRed := codRed ;
+      PiRedTy.codExt := codExt
+        |} in
+  let ΠA' : PiRedTy Γ A' := {|
+    PiRedTy.na := na' ; PiRedTy.dom := dom' ;
+    PiRedTy.cod := cod' ;
+    PiRedTy.red := red' ;
+    PiRedTy.domTy := domTy' ;
+    PiRedTy.codTy := codTy' ;
+    PiRedTy.domRed := domRed' ;
+    PiRedTy.codRed := codRed' ;
+    PiRedTy.codExt := codExt'
+      |} in
+  forall t, [Γ ||-Π t : A | ΠA] -> [Γ ||-Π t : A' | ΠA'].
+Proof.
+  intros IHdom IHcod ΠA ΠA' B [] ; cbn in *.
+  econstructor.
+  1-3: now mltt.
+  - intros.
+    unshelve eapply IHcod.
+    2: now auto.
+    now apply IHdom.
+  - intros.
+    unshelve eapply IHcod, eq.
+    all: now eapply IHdom.
+Qed.
+
+Lemma ΠIrrelevanceTmEq Γ A na dom cod A' na' dom' cod'
+  (domTy : [Γ |- dom])
+  (codTy : [Γ,, vass na dom |- cod])
+  (red : [Γ |- A :⇒*: tProd na dom cod])
+  (domRed : forall Δ : context, [  |- Δ] -> LRPack Δ dom)
+  (codRed : forall (Δ : context) (a : term) (h : [  |- Δ]),
+            [domRed Δ h | Δ ||- a : dom] -> LRPack Δ (cod {0 := a}))
+  (codExt : forall (Δ : context) (a b : term) (h : [  |- Δ])
+              (ha : [domRed Δ h | Δ ||- a : dom]),
+            [domRed Δ h | Δ ||- b : dom] ->
+            [domRed Δ h | Δ ||- a ≅ b : dom] ->
+            [codRed Δ a h ha | Δ ||- cod{0 := a} ≅ cod{0 := b}])
+  (domTy': [Γ |- dom'])
+  (codTy': [Γ,, vass na' dom' |- cod'])
+  (red': [Γ |- A' :⇒*: tProd na' dom' cod'])
+  (domRed': forall Δ : context, [  |- Δ] -> LRPack Δ dom')
+  (codRed': forall (Δ : context) (a : term) (h : [  |- Δ]),
+            [domRed' Δ h | Δ ||- a : dom'] -> LRPack Δ (cod' {0 := a}))
+  (codExt': forall (Δ : context) (a b : term) (h : [  |- Δ])
+              (ha : [domRed' Δ h | Δ ||- a : dom']),
+            [domRed' Δ h | Δ ||- b : dom'] ->
+            [domRed' Δ h | Δ ||- a ≅ b : dom'] ->
+            [codRed' Δ a h ha | Δ ||- cod'{0 := a} ≅ cod'{0 := b}])
+  (eqPi : [Γ |- tProd na dom cod ≅ tProd na' dom' cod']) :
+  
+  (forall (Δ : context) (h : [  |- Δ]),
+  [× (forall B : term,
+      [domRed Δ h | Δ ||- dom ≅ B] <-> [domRed' Δ h | Δ ||- dom' ≅ B]),
+    (forall t : term,
+      [domRed Δ h | Δ ||- t : dom] <-> [domRed' Δ h | Δ ||- t : dom']) &
+    (forall t u : term,
+      [domRed Δ h | Δ ||- t ≅ u : dom ] <-> [domRed' Δ h | Δ ||- t ≅ u : dom'])]) ->
+  (forall (Δ : context) (a : term) (h : [  |- Δ])
+      (ha : [domRed Δ h | Δ ||- a : dom])
+      (ha' : [domRed' Δ h | Δ ||- a : dom']),
+  [× (forall B : term,
+      [codRed Δ a h ha | Δ ||- cod{0 := a} ≅ B] <->
+      [codRed' Δ a h ha' | Δ ||- cod'{0 := a} ≅ B]),
+    (forall t : term,
+      [codRed Δ a h ha | Δ ||- t : cod{0 := a} ] <->
+      [codRed' Δ a h ha' | Δ ||- t : cod'{0 := a} ]) &
+    (forall t u : term,
+      [codRed Δ a h ha | Δ ||- t ≅ u : cod{0 := a} ] <->
+      [codRed' Δ a h ha' | Δ ||- t ≅ u : cod'{0 := a} ])]) ->
+  let ΠA : PiRedTy Γ A := {|
+      PiRedTy.na := na ; PiRedTy.dom := dom ;
+      PiRedTy.cod := cod ;
+      PiRedTy.red := red ;
+      PiRedTy.domTy := domTy ;
+      PiRedTy.codTy := codTy ;
+      PiRedTy.domRed := domRed ;
+      PiRedTy.codRed := codRed ;
+      PiRedTy.codExt := codExt
+       |} in
+  let ΠA' : PiRedTy Γ A' := {|
+    PiRedTy.na := na' ; PiRedTy.dom := dom' ;
+    PiRedTy.cod := cod' ;
+    PiRedTy.red := red' ;
+    PiRedTy.domTy := domTy' ;
+    PiRedTy.codTy := codTy' ;
+    PiRedTy.domRed := domRed' ;
+    PiRedTy.codRed := codRed' ;
+    PiRedTy.codExt := codExt'
+     |} in
+  forall t u, [Γ ||-Π t ≅ u : A | ΠA] -> [Γ ||-Π t ≅ u : A' | ΠA'].
+Proof.
+  intros IHdom IHcod ΠA ΠA' t u [] ; cbn in *.
+  unshelve econstructor.
+  - now eapply ΠIrrelevanceTm.
+  - now eapply ΠIrrelevanceTm.
+  - cbn.
+    mltt.
+  - intros.
+    unshelve eapply IHcod.
+    2: now auto.
+    now apply IHdom.
+Qed.
+
+Theorem LRIrrelevant Γ A A' {lA eqTyA redTmA eqTmA lA' eqTyA' redTmA' eqTmA'}
+    (lrA : LRl lA Γ A eqTyA redTmA eqTmA) (lrA' : LRl lA' Γ A' eqTyA' redTmA' eqTmA') :
+    eqTyA A' ->
+    [× forall B, eqTyA B <-> eqTyA' B ,
+    forall t, redTmA t <-> redTmA' t &
+    forall t u, eqTmA t u <-> eqTmA' t u ].
+Proof.
+  intros he.
+  set (s := ShapeViewConv lrA lrA' he).
+  induction lrA as [? [? []] | ? ? [] | ? A [] [] IHdom IHcod]
+    using LR_rect in lA', A', eqTyA', eqTmA', redTmA', lrA', he, s |- *.
+  - destruct lrA' as [? [? []] | | ]; try solve [destruct s] ; clear s.
+    split.
+    + intros ?.
+      split.
+      all: eauto.
+    + intros ?.
+      split.
+      all: intros [].
+      all: now econstructor.
+    + intros ? ?.
+      split.
+      all: intros [[] []].
+      all: unshelve econstructor ; tea.
+      1-4: now econstructor.
+      all: eassumption.
+  - destruct lrA' as [|? A' neA'|] ; try solve [destruct s] ; clear s.
+    destruct he as [AA], neA' as [AA'] ; cbn in *.
+    assert (AA' = AA) as ->
+      by (eapply nred_det_ty ; mltt).
+    split.
+    + intros ?.
+      split.
+      all: intros [].
+      all: econstructor.
+      all: now mltt.
+    + intros ?.
+      split.
+      all: intros [].
+      all: econstructor.
+      all: now mltt.
+    + intros ? ?.
+      split.
+      all: intros [].
+      all: econstructor.
+      all: cbn in *.
+      1-2,6-7: now eapply TermRedWFConv ; mltt.
+      1-2,4-5: eassumption.
+      all: assert [Γ |- A ≅ A'] by (eapply TypeTrans ; mltt).
+      all: now mltt.
+  - destruct lrA' as [| | ? A' [] []] ; try solve [destruct s] ; clear s.
+    destruct he ; cbn -[subst1] in *.
+    assert (redPi0 = redPi1) as ePi
+      by (eapply nred_det_ty ; mltt).
+    subst redPi redPi0 redPi1.
+    inversion ePi ; subst ; clear ePi.
+    pose proof (IHdom_ := fun Δ h => IHdom Δ h _ _ _ _ _ (domAd0 Δ h) (domRed1 Δ h)).
+    assert (IHcod_ : forall Δ a (h : [ |- Δ])
+      (ha : [domRed Δ h | Δ ||- a : dom])
+      (ha' : [domRed0 Δ h | Δ ||- a : dom1]),
+      [×
+        (forall B,
+          [codRed Δ a h ha | Δ ||- cod{0 := a} ≅ B] <->
+          [codRed0 Δ a h ha' | Δ ||- cod1{0 := a} ≅ B]),
+        (forall t,
+          [codRed Δ a h ha | Δ ||- t : cod{0 := a}] <->
+          [codRed0 Δ a h ha' | Δ ||- t : cod1{0 := a}]) &
+      (forall t u,
+        [codRed Δ a h ha | Δ ||- t ≅ u : cod{0 := a}] <->
+        [codRed0 Δ a h ha' | Δ ||- t ≅ u : cod1{0 := a}])
+      ]).
+    {
+      intros.
+      eapply IHcod.
+      1: eapply codAd0.
+      eauto.
+    }
+    split.
+    + split ; intros.
+      all: eapply ΠIrrelevanceTyEq.
+      4,8: eassumption.
+      1,4: mltt.
+      1-2: now eauto.
+      * do 2 split ; intros.
+        all: now eapply IHdom_ ; eauto.
+      * do 2 split ; intros.
+        all: now eapply IHcod_ ; eauto.
+    + split ; intros.
+      all: eapply ΠIrrelevanceTm.
+      4,8: eassumption.
+      1,4: mltt.
+      1-2: now eauto.
+      * do 2 split ; intros.
+        all: now eapply IHdom_ ; eauto.
+      * do 2 split ; intros.
+        all: now eapply IHcod_ ; eauto.
+    + split ; intros.
+      all: eapply ΠIrrelevanceTmEq.
+      4,8: eassumption.
+      1,4: mltt.
+      1-2: now eauto.
+      * do 2 split ; intros.
+        all: now eapply IHdom_ ; eauto.
+      * do 2 split ; intros.
+        all: now eapply IHcod_ ; eauto.
+Qed.
+
+Corollary TyEqIrrelevant Γ A {lA eqTyA redTmA eqTmA lA' eqTyA' redTmA' eqTmA'}
+  (lrA : LRl lA Γ A eqTyA redTmA eqTmA) (lrA' : LRl lA' Γ A eqTyA' redTmA' eqTmA') :
+  forall B, eqTyA B -> eqTyA' B.
+Proof.
+  apply (LRIrrelevant _ _ _ lrA lrA').
+  now eapply LRTyEqRefl.
+Qed.
+
+Corollary LRTyEqIrrelevant lA lA' Γ A (lrA : [Γ ||-< lA > A]) (lrA' : [Γ ||-< lA'> A]) :
+  forall B, [Γ ||-< lA > A ≅ B | lrA] -> [Γ ||-< lA' > A ≅ B | lrA'].
+Proof.
+  destruct lrA, lrA'.
+  cbn in *.
+  now eapply TyEqIrrelevant.
+Qed.
+
+Corollary RedTmIrrelevant Γ A {lA eqTyA redTmA eqTmA lA' eqTyA' redTmA' eqTmA'}
+  (lrA : LRl lA Γ A eqTyA redTmA eqTmA) (lrA' : LRl lA' Γ A eqTyA' redTmA' eqTmA') :
+  forall t, redTmA t -> redTmA' t.
+Proof.
+  apply (LRIrrelevant _ _ _ lrA lrA').
+  now eapply LRTyEqRefl.
+Qed.
+
+Corollary LRTmRedIrrelevant lA lA' Γ A (lrA : [Γ ||-< lA > A]) (lrA' : [Γ ||-< lA'> A]) :
+  forall t, [Γ ||-< lA > t : A | lrA] -> [Γ ||-< lA' > t : A | lrA'].
+Proof.
+  destruct lrA, lrA'.
+  cbn in *.
+  now eapply RedTmIrrelevant.
+Qed.
+
+Corollary TmEqIrrelevant Γ A {lA eqTyA redTmA eqTmA lA' eqTyA' redTmA' eqTmA'}
+  (lrA : LRl lA Γ A eqTyA redTmA eqTmA) (lrA' : LRl lA' Γ A eqTyA' redTmA' eqTmA') :
+  forall t u, eqTmA t u -> eqTmA' t u.
+Proof.
+  apply (LRIrrelevant _ _ _ lrA lrA').
+  now eapply LRTyEqRefl.
+Qed.
+
+Corollary LRTmEqIrrelevant lA lA' Γ A (lrA : [Γ ||-< lA > A]) (lrA' : [Γ ||-< lA'> A]) :
+  forall t u, [Γ ||-< lA > t ≅ u : A | lrA] -> [Γ ||-< lA' > t ≅ u : A | lrA'].
+Proof.
+  destruct lrA, lrA'.
+  cbn in *.
+  now eapply TmEqIrrelevant.
+Qed.
+
+
+Corollary TyEqSym Γ A A' {lA eqTyA redTmA eqTmA lA' eqTyA' redTmA' eqTmA'}
+  (lrA : LRl lA Γ A eqTyA redTmA eqTmA) (lrA' : LRl lA' Γ A' eqTyA' redTmA' eqTmA') :
+  eqTyA A' -> eqTyA' A.
+Proof.
+  intros.
+  apply (LRIrrelevant _ _ _ lrA lrA').
+  1: eauto.
+  now eapply LRTyEqRefl.
+Qed.
+
+Corollary LRTyEqSym lA lA' Γ A A' (lrA : [Γ ||-< lA > A]) (lrA' : [Γ ||-< lA'> A']) :
+  [Γ ||-< lA > A ≅ A' | lrA] -> [Γ ||-< lA' > A' ≅ A | lrA'].
+Proof.
+  destruct lrA, lrA'.
+  cbn in *.
+  now eapply TyEqSym.
+Qed.
+
+Corollary RedTmConv Γ A A' {lA eqTyA redTmA eqTmA lA' eqTyA' redTmA' eqTmA'}
+  (lrA : LRl lA Γ A eqTyA redTmA eqTmA) (lrA' : LRl lA' Γ A' eqTyA' redTmA' eqTmA') :
+  eqTyA A' ->
+  forall t, redTmA t -> redTmA' t.
+Proof.
+  apply (LRIrrelevant _ _ _ lrA lrA').
+Qed.
+
+Corollary LRTmRedConv lA lA' Γ A A' (lrA : [Γ ||-< lA > A]) (lrA' : [Γ ||-< lA'> A' ]) :
+  [Γ ||-< lA > A ≅ A' | lrA ] ->
+  forall t, [Γ ||-< lA > t : A | lrA] -> [Γ ||-< lA' > t : A' | lrA'].
+Proof.
+  destruct lrA, lrA'.
+  cbn in *.
+  now eapply RedTmConv.
+Qed.
+
+Corollary TmEqRedConv Γ A A' {lA eqTyA redTmA eqTmA lA' eqTyA' redTmA' eqTmA'}
+  (lrA : LRl lA Γ A eqTyA redTmA eqTmA) (lrA' : LRl lA' Γ A' eqTyA' redTmA' eqTmA') :
+  eqTyA A' ->
+  forall t u, eqTmA t u -> eqTmA' t u.
+Proof.
+  apply (LRIrrelevant _ _ _ lrA lrA').
+Qed.
+
+Corollary LRTmEqRedConv lA lA' Γ A A' (lrA : [Γ ||-< lA > A]) (lrA' : [Γ ||-< lA'> A']) :
+  [Γ ||-< lA > A ≅ A' | lrA ] ->
+  forall t u, [Γ ||-< lA > t ≅ u : A | lrA] -> [Γ ||-< lA' > t ≅ u : A' | lrA'].
+Proof.
+  destruct lrA, lrA'.
+  cbn in *.
+  now eapply TmEqRedConv.
+Qed.
