theories/LRInduction.v
@@ -1,60 +1,7 @@
 From MetaCoq.PCUIC Require Import PCUICAst.
 From LogRel Require Import Notations Untyped MLTTTyping LogicalRelation.
 
-Set Universe Polymorphism.
-
-Theorem LR_rect0
-  (rec : forall l', l' << zero -> LogRelKit)
-  (P : forall {c t rEq rTe rTeEq}, LR rec c t rEq rTe rTeEq  -> Type) :
-  (forall (Γ : context) (A : term) (neA : [Γ ||-ne A]),
-    P (LRne rec neA)) ->
-
-  (forall (Γ : context) (A : term) (ΠA : [ Γ ||-Πd A ]) (HAad : PiRedTyAdequate (LR rec) ΠA),
-    (forall {Δ} (h : [ |- Δ]),
-      P (HAad.(PiRedTy.domAd) h)) ->
-    (forall {Δ a} (h1 : [ |- Δ ]) 
-      (h2 : [ ΠA.(PiRedTy.domRed) h1 | Δ ||- a : ΠA.(PiRedTy.dom) ]),
-      P (HAad.(PiRedTy.codAd) h1 h2)) ->
-    P (LRPi rec ΠA HAad)) ->
-
-  forall (c : context) (t : term) (rEq rTe : term -> Type)
-    (rTeEq  : term -> term -> Type) (lr : LR rec c t rEq rTe rTeEq), 
-   P lr.
-Proof.
-  intros Hne HPi.
-  fix HRec 6.
-  intros c t rEq rTE rTeEq lr.
-  case lr.
-  - destruct H as [? l_].
-    inversion l_.
-  - eapply Hne.
-  - destruct ΠAad ; unfold LRPackAdequate in * ; cbn in *.
-    eapply HPi.
-    all: intros ; eapply HRec.
-Qed.
-
-Theorem LR_rect0'
-  (P : forall {c t rEq rTe rTeEq}, @LR zero rec0 c t rEq rTe rTeEq  -> Type) :
-  (forall (Γ : context) (A : term) (neA : [Γ ||-ne A]),
-    P (LRne rec0 neA)) ->
-
-  (forall (Γ : context) (A : term) (ΠA : [ Γ ||-Πd A ]) (HAad : PiRedTyAdequate (LR rec0) ΠA),
-    (forall {Δ} (h : [ |- Δ]),
-      P (HAad.(PiRedTy.domAd) h)) ->
-    (forall {Δ a} (h1 : [ |- Δ ]) 
-      (h2 : [ ΠA.(PiRedTy.domRed) h1 | Δ ||- a : ΠA.(PiRedTy.dom) ]),
-      P (HAad.(PiRedTy.codAd) h1 h2)) ->
-    P (LRPi rec0 ΠA HAad)) ->
-
-  forall (Γ : context) (A : term) (lr : [Γ ||-< zero > A]),
-  P (lr.(LRAd.adequate)).
-Proof.
-  intros.
-  eapply LR_rect0.
-  all: eassumption.
-Qed.
-
-Fixpoint LR_embedding {l l'} (l_ : l << l')
+#[universes(polymorphic)]Fixpoint LR_embedding {l l'} (l_ : l << l')
   {Γ A rEq rTe rTeEq} (lr : LRl l Γ A rEq rTe rTeEq) {struct lr} : (LRl l' Γ A rEq rTe rTeEq) :=
   match lr with
    | LRU Γ H =>
@@ -73,12 +20,13 @@ Fixpoint LR_embedding {l l'} (l_ : l << l')
       |}
   end.
 
-Theorem LR_rect1
-  (rec : forall l', l' << one -> LogRelKit)
+#[universes(polymorphic)]Theorem LR_rect
+  (l : TypeLevel)
+  (rec : forall l', l' << l -> LogRelKit)
   (P : forall {c t rEq rTe rTeEq},
-  @LR one rec c t rEq rTe rTeEq  -> Type) :
+    LR rec c t rEq rTe rTeEq  -> Type) :
 
-  (forall (Γ : context) (h : [Γ ||-U one]),
+  (forall (Γ : context) (h : [Γ ||-U l]),
     P (LRU rec h)) ->
 
   (forall (Γ : context) (A : term) (neA : [Γ ||-ne A]),
@@ -106,7 +54,42 @@ Proof.
     all: intros ; eapply HRec.
 Qed.
 
-Theorem LR_rect (P : forall {l Γ A}, [Γ ||-< l > A] -> Type) :
+Theorem LR_rect_LogRelRec
+  (P : forall {l Γ t rEq rTe rTeEq},
+  LRl l Γ t rEq rTe rTeEq  -> Type) :
+
+  (forall (Γ : context) (h : [Γ ||-U one]),
+    P (LRU (rec1) h)) ->
+
+  (forall (l : TypeLevel) (Γ : context) (A : term) (neA : [Γ ||-ne A]),
+    P (LRne (LogRelRec l) neA)) ->
+
+  (forall (l : TypeLevel) (Γ : context) (A : term) (ΠA : [ Γ ||-Πd A ])
+    (HAad : PiRedTyAdequate (LRl l) ΠA),
+  (forall {Δ} (h : [ |- Δ]),
+    P (HAad.(PiRedTy.domAd) h)) ->
+  (forall {Δ a} (h1 : [ |- Δ ]) 
+    (h2 : [ ΠA.(PiRedTy.domRed) h1 | Δ ||- a : ΠA.(PiRedTy.dom) ]),
+  P (HAad.(PiRedTy.codAd) h1 h2)) ->
+  P (LRPi (LogRelRec l) ΠA HAad)) ->
+
+  forall (l : TypeLevel) (c : context) (t : term) (rEq rTe : term -> Type)
+    (rTeEq  : term -> term -> Type) (lr : LR (LogRelRec l) c t rEq rTe rTeEq),
+    P lr.
+Proof.
+  intros.
+  apply LR_rect.
+  - intros.
+    destruct l.
+    2: auto.
+    destruct h as [? lt].
+    inversion lt.
+  - auto.
+  - auto.
+Qed.
+
+Theorem LR_rect_TyUr
+  (P : forall {l Γ A}, [Γ ||-< l > A] -> Type) :
 
   (forall (Γ : context) (h : [Γ ||-U one]),
     P (LRU_ h)) ->
@@ -125,87 +108,7 @@ Theorem LR_rect (P : forall {l Γ A}, [Γ ||-< l > A] -> Type) :
   forall (l : TypeLevel) (Γ : context) (A : term) (lr : [Γ ||-< l > A]),
     P lr.
 Proof.
-  intros HU Hne HPi [] Γ A lr.
-  - apply (LR_rect0 rec0 (fun Γ A _ _ _ lr => P zero Γ A (LRbuild lr))).
-    + intros.
-      apply Hne.
-    + intros.
-      apply HPi ; try eassumption.
-  - apply (LR_rect1 rec1 (fun Γ A _ _ _ lr => P one Γ A (LRbuild lr))).
-    + assumption.
-    + intros.
-      apply Hne.
-    + intros.
-      apply HPi.
-      all: eassumption.
-Qed.
-
-Theorem LR_rec (P : RedRel) :
-  (forall (Γ : context) (A : term) (neA : [Γ ||-ne A]),
-  P Γ A (fun B : term => [Γ ||-ne A ≅ B | neA])
-  (fun t : term => [Γ ||-ne t : A | neA])
-  (fun t u : term => [Γ ||-ne t ≅ u : A | neA])) ->
-
-  (forall (Γ : context) (A : term) (ΠA : [ Γ ||-Πd A ])
-  (HAad : {l & PiRedTyAdequate (LRl l) ΠA}),
-  (forall {Δ} (h : [ |- Δ]),
-    P Δ (PiRedTy.dom ΠA) (LRPack.eqTy (PiRedTy.domRed ΠA h))
-    (LRPack.redTm (PiRedTy.domRed ΠA h)) (LRPack.eqTm (PiRedTy.domRed ΠA h))) ->
-  (forall {Δ a} (h1 : [ |- Δ ]) 
-    (h2 : [ ΠA.(PiRedTy.domRed) h1 | Δ ||- a : ΠA.(PiRedTy.dom) ]),
-    P Δ ((PiRedTy.cod ΠA) {0 := a}) (LRPack.eqTy (PiRedTy.codRed ΠA h1 h2))
-    (LRPack.redTm (PiRedTy.codRed ΠA h1 h2))
-    (LRPack.eqTm (PiRedTy.codRed ΠA h1 h2))) ->
-  P Γ A (fun B : term => [Γ ||-Π A ≅ B | ΠA])
-  (fun t : term => [Γ ||-Π t : A | ΠA])
-  (fun t u : term => [Γ ||-Π t ≅ u : A | ΠA])) ->
-
-  (forall (Γ : context) (h : [Γ ||-U one ]),
-  P Γ U (fun B : term => [Γ ||-U≅ B])
-  (fun t : term => [rec1 | Γ ||-U t :U | h])
-  (fun t u : term => [rec1 | Γ ||-U t ≅ u :U | h])) ->
-
-  forall (l : TypeLevel) (Γ : context) (t : term) (rEq rTe : term -> Type)
-  (rTeEq  : term -> term -> Type) (lr : LR (LogRelRec l) Γ t rEq rTe rTeEq),
-  P Γ t rEq rTe rTeEq.
-Proof.
-  intros Hne HPi HU [].
-  - apply LR_rect0.
-    + assumption.
-    + intros.
-      apply HPi ; try eassumption.
-      exists zero.
-      eassumption.
-  - apply LR_rect1.
-    + assumption.
-    + assumption.
-    + intros.
-      apply HPi ; try eassumption.
-      exists one.
-      eassumption.
-Qed.
-
-Theorem LR_rec' (P : context -> term -> Type) :
-  (forall (Γ : context) (A : term) (neA : [Γ ||-ne A]),
-  P Γ A) ->
-
-  (forall (Γ : context) (A : term) (ΠA : [ Γ ||-Πd A ])
-    (HAad : {l & PiRedTyAdequate (LRl l) ΠA}),
-    (forall {Δ} (h : [ |- Δ]),
-      P Δ (PiRedTy.dom ΠA)) ->
-    (forall {Δ a} (h1 : [ |- Δ ]) 
-      (h2 : [ ΠA.(PiRedTy.domRed) h1 | Δ ||- a : ΠA.(PiRedTy.dom) ]),
-      P Δ ((PiRedTy.cod ΠA) {0 := a})) ->
-    P Γ A) ->
-
-  (forall (Γ : context) (h : [Γ ||-U one ]),
-    P Γ U) ->
-
-  forall (l : TypeLevel) (Γ : context) (A : term),
-    [Γ ||-< l > A] -> P Γ A.
-Proof.
-  intros Hne HPi HU l Γ A [[] lr].
-  red in lr ; cbn in lr.
-  eapply (LR_rec (fun Γ A _ _ _ => P Γ A)).
-  all: eassumption.
+  intros HU Hne HPi l Γ A lr.
+  apply (LR_rect_LogRelRec (fun l Γ A _ _ _ lr => P l Γ A (LRbuild lr))).
+  all: auto.
 Qed.
