theories/Utils.v
@@ -1,0 +1,6 @@
+From MetaCoq Require Import utils.
+
+Definition iff (A B : Type) :=
+  (A -> B) × (B -> A).
+
+Notation "A <-> B" := (iff A B) : type_scope.
